theories/program_logic/itreewp.v
@@ -12,11 +12,11 @@ Section itreewp.
 Definition command_predicate {V R} (c: envE V R) (σ σ': gmap loc V): R -> Prop.
 refine (
   match c with
-  | GetE l       => λ v, σ !! l = Some v /\ σ' = σ 
-  | PutE l v'    => λ _, is_Some (σ !! l) /\ σ' = <[l := v']> σ
-  | AllocE v'    => λ l, l = fresh_loc σ /\ σ' = <[l := v']> σ
-  | FreeE l      => λ _, is_Some (σ !! l) /\ σ' = delete l σ
-  | CasE l v1 v2 => λ '(vret, upd), if upd then σ !! l = Some v1 /\ vret = v1 /\ σ' = <[l := v2]> σ  
+  | GetE l           => λ v, σ !! l = Some v /\ σ' = σ 
+  | PutE l v'        => λ _, is_Some (σ !! l) /\ σ' = <[l := v']> σ
+  | AllocE v'        => λ l, l = fresh_loc σ /\ σ' = <[l := v']> σ
+  | FreeE l          => λ _, is_Some (σ !! l) /\ σ' = delete l σ
+  | CmpXchgE l v1 v2 => λ '(vret, upd), if upd then σ !! l = Some v1 /\ vret = v1 /\ σ' = <[l := v2]> σ  
                                    else ∃x, σ !! l = Some x /\ vret = x /\ σ = σ' /\ x ≠ v1
   end
 ).
@@ -559,7 +559,7 @@ Section heap_wp.
   Lemma wp_cas_suc l v1 v2 E (Φ: (nat * bool) -> iProp Σ):
     points_to γ l v1
     -∗ ▷(points_to γ l v2  -∗ Φ (v1, true))
-    -∗ wp (state_interp γ) E (itree.cas l v1 v2) Φ.
+    -∗ wp (state_interp γ) E (itree.cmpXchg l v1 v2) Φ.
   Proof.
     iIntros "Hpt HPost".
     rewrite wp_unfold. unfold wp_pre.
@@ -580,7 +580,7 @@ Section heap_wp.
     ⌜v1 <> v3⌝ -∗
     points_to γ l v1
     -∗ ▷(points_to γ l v1  -∗ Φ (v1, false))
-    -∗ wp (state_interp γ) E (itree.cas l v3 v2) Φ.
+    -∗ wp (state_interp γ) E (itree.cmpXchg l v3 v2) Φ.
   Proof.
     iIntros "%Hneq Hpt HPost".
     rewrite wp_unfold. unfold wp_pre.
